wip

theories/gitree/reify.v
@@ -2,62 +2,86 @@ From iris.proofmode Require Import classes tactics.
 From gitrees Require Import prelude.
 From gitrees.gitree Require Import core.
 
-Section abstract_res.
-  Variable (R : Type).
-  Variable (Op : R → Type).
-  Variable (In : forall {r : R}, Op r → oFunctor).
-  Variable (Out : forall {r : R}, Op r → oFunctor).
-  Variable (St : R → oFunctor).
+Section reifiers.
+  #[local] Open Scope type.
 
-  Definition reifier_type (r : R) : Type :=
-    forall (op : Op r) {X} `{!Cofe X},
-      ((In op ♯ X) * (St r ♯ X) -n> (Out op ♯ X) * (St r ♯ X))%type.
+  (** A single reifier *)
+  Record sReifier :=
+    { sReifier_ops : opsInterp;
+      sReifier_state : oFunctor;
+      sReifier_re {X} `{!Cofe X} : forall (op : opid sReifier_ops),
+          (Ins (sReifier_ops op) ♯ X) * (sReifier_state ♯ X)
+              -n> optionO ((Outs (sReifier_ops op) ♯ X) * (sReifier_state ♯ X));
+      sReifier_inhab :: Inhabited (sReifier_state ♯ unitO);
+      sReifier_cofe X (HX : Cofe X) :: Cofe (sReifier_state ♯ X);
+    }.
 
-  Variable (Re : forall r, reifier_type r).
+  (** Global reifiers: a collection of reifiers *)
+  Inductive gReifiers : nat → Type :=
+  | gReifiers_nil : gReifiers 0
+  | gReifiers_cons {n} : sReifier → gReifiers n → gReifiers (S n)
+  .
 
-  Inductive hvec : nat → Type :=
-  | nil : hvec 0
-  | cons {n} : R → hvec n → hvec (S n).
-
-  Definition hvec_S_inv {n} (P : hvec (S n) → Type)
-    (Hcons : ∀ sR v, P (cons sR v)) v : P v.
+  Definition grs_S_inv {n} (P : gReifiers (S n) → Type)
+    (Hcons : ∀ sR v, P (gReifiers_cons sR v)) v : P v.
   Proof.
     revert P Hcons.
-    refine match v with nil => tt
-                      | cons sR v => λ P Hcons, Hcons sR v end.
+    refine match v with gReifiers_nil => tt
+                      | gReifiers_cons sR v => λ P Hcons, Hcons sR v end.
   Defined.
 
-  Global Instance hvec_lookup_total : ∀ m, LookupTotal (fin m) R (hvec m) :=
+  Global Instance gReifiers_lookup_total : ∀ m, LookupTotal (fin m) sReifier (gReifiers m) :=
   fix go m i {struct i} := let _ : ∀ m, LookupTotal _ _ _ := @go in
-  match i in fin m return hvec m → R with
-  | 0%fin => hvec_S_inv (λ _, R) (λ x _, x)
-  | FS j => hvec_S_inv (λ _, R) (λ _ v, v !!! j)
+  match i in fin m return gReifiers m → sReifier with
+  | 0%fin => grs_S_inv (λ _, sReifier) (λ x _, x)
+  | FS j => grs_S_inv (λ _, sReifier) (λ _ v, v !!! j)
   end.
 
-  (** global signature *)
-  Definition glob_Op {n} (rs : hvec n) : Type :=
-    { i : fin n & Op (rs !!! i) }.
-  Definition glob_In {n} {rs : hvec n} : glob_Op rs → oFunctor :=
-    λ iop, @In (rs !!! projT1 iop) (projT2 iop).
-  Definition glob_Out {n} {rs : hvec n} : glob_Op rs → oFunctor :=
-    λ iop, @Out (rs !!! projT1 iop) (projT2 iop).
+  Program Definition gReifiers_ops {n} (rs : gReifiers n) : opsInterp :=
+    {| opid := { i : fin n & opid (sReifier_ops (rs !!! i)) };
+       opsInterp_lookup := λ iop, sReifier_ops (rs !!! projT1 iop) (projT2 iop)
+    |}.
+  Next Obligation.
+    intros n rs.
+    unfold EqDecision. intros [i1 x1] [i2 x2].
+    unfold Decision.
+    destruct (decide (i1 = i2)) as [<-|Hi].
+    - destruct (decide (x1 = x2)) as [<-|Hx].
+      + left. reflexivity.
+      + right. naive_solver.
+    - right. naive_solver.
+  Qed.
 
-  Fixpoint glob_St {n} (rs : hvec n) : oFunctor :=
+  Fixpoint gReifiers_state {n} (rs : gReifiers n) : oFunctor :=
     match rs with
-    | nil => unitO
-    | cons r rs => St r * glob_St rs
-    end%OF.
-
-  Fixpoint glob_St_rest {n} (i : fin n) : hvec n → oFunctor :=
-    match i in fin n return hvec n → oFunctor with
-    | 0%fin => hvec_S_inv (λ _, oFunctor)
-                 (λ _ rs, glob_St rs)
-    | FS j => hvec_S_inv (λ _, oFunctor)
-                 (λ r rs, St r * glob_St_rest j rs)%OF
+    | gReifiers_nil => unitO
+    | gReifiers_cons sR rs => sReifier_state sR * (gReifiers_state rs)
     end.
 
-  Lemma glob_St_decomp' {m} (i : fin m) (rs : hvec m) {X} `{!Cofe X} :
-    ofe_iso (glob_St rs ♯ X) ((St (rs !!! i) ♯ X) * (glob_St_rest i rs ♯ X))%type.
+  #[export] Instance reifiers_state_cofe {n} (rs : gReifiers n) X `{!Cofe X} :
+    Cofe (gReifiers_state rs ♯ X).
+  Proof.
+    induction rs; simpl; first apply _.
+    destruct s. apply _.
+  Qed.
+  #[export] Instance reifiers_state_inhab {n} (rs : gReifiers n) :
+    Inhabited (gReifiers_state rs ♯ unitO).
+  Proof.
+    induction rs; simpl; first apply _.
+    destruct s. apply _.
+  Qed.
+
+  Fixpoint gState_rest {m} (i : fin m) : gReifiers m → oFunctor :=
+    match i in fin m return gReifiers m → oFunctor with
+    | 0%fin => grs_S_inv (λ _, oFunctor)
+                 (λ sR rs, gReifiers_state rs)
+    | FS j => grs_S_inv (λ _, oFunctor)
+                 (λ sR rs, sReifier_state sR * gState_rest j rs)%OF
+    end.
+
+  Lemma gState_decomp' {m} (i : fin m) (rs : gReifiers m) {X} `{!Cofe X} :
+    ofe_iso (gReifiers_state rs ♯ X)
+            ((sReifier_state (rs !!! i) ♯ X) * (gState_rest i rs ♯ X))%type.
   Proof.
     revert i. induction rs as [|n r rs]=>i.
     { inversion i. }
@@ -75,563 +99,147 @@ Section abstract_res.
     - intros (s & x & rest). simpl. repeat f_equiv; rewrite ofe_iso_12//.
     - intros (x & rest). simpl. f_equiv.
       rewrite -surjective_pairing. apply ofe_iso_21.
-  Qed.
-  Definition glob_St_decomp {m} (i : fin m) {rs : hvec m} {X} `{!Cofe X} :
-    (glob_St rs ♯ X) -n> ((St (rs !!! i) ♯ X) * (glob_St_rest i rs ♯ X))%type
-    := ofe_iso_1 (glob_St_decomp' i rs).
-  Program Definition glob_St_recomp {m} {i : fin m} {rs : hvec m} {X} `{!Cofe X} :
-    (glob_St_rest i rs ♯ X) -n> (St (rs !!! i) ♯ X) -n> (glob_St rs ♯ X)
-    := λne rest st, ofe_iso_2 (glob_St_decomp' i rs) (st, rest).
+  Defined.
+  Definition gState_decomp {m} (i : fin m) {rs : gReifiers m} {X} `{!Cofe X} :
+    (gReifiers_state rs ♯ X) -n> ((sReifier_state (rs !!! i) ♯ X) * (gState_rest i rs ♯ X))%type
+    := ofe_iso_1 (gState_decomp' i rs).
+  Program Definition gState_recomp {m} {i : fin m} {rs : gReifiers m} {X} `{!Cofe X} :
+    (gState_rest i rs ♯ X) -n> (sReifier_state (rs !!! i) ♯ X) -n> (gReifiers_state rs ♯ X)
+    := λne rest st, ofe_iso_2 (gState_decomp' i rs) (st, rest).
   Solve All Obligations with solve_proper_please.
 
-  Lemma glob_St_decomp_recomp {m} (i : fin m) {rs : hvec m} {X} `{!Cofe X}
-    (σ : St (rs !!! i) ♯ X) rest :
-    glob_St_decomp i (glob_St_recomp rest σ) ≡ (σ, rest).
+  Lemma gState_decomp_recomp {m} (i : fin m) {rs : gReifiers m} {X} `{!Cofe X}
+    (σ : sReifier_state (rs !!! i) ♯ X) rest :
+    gState_decomp i (gState_recomp rest σ) ≡ (σ, rest).
   Proof. rewrite ofe_iso_12. reflexivity. Qed.
+  Opaque gState_recomp gState_decomp.
 
-  Definition glob_Re {n} {rs : hvec n} (op : glob_Op rs) {X} `{!Cofe X} :
-    (glob_In op ♯ X) * (glob_St rs ♯ X) → (glob_Out op ♯ X) * (glob_St rs ♯ X)
-    :=  λ xst,
+  Program Definition gReifiers_re {n} (rs : gReifiers n) {X} `{!Cofe X}
+    (op : opid (gReifiers_ops rs)) :
+    (Ins (gReifiers_ops rs op) ♯ X) * (gReifiers_state rs ♯ X) -n>
+      optionO ((Outs (gReifiers_ops rs op) ♯ X) * (gReifiers_state rs ♯ X))
+    :=  λne xst,
       let  i := projT1 op in
       let op' := projT2 op in
       let x := xst.1 in
       let st := xst.2 in
-      let fs := glob_St_decomp i st in
+      let fs := gState_decomp i st in
       let σ := fs.1 in
       let rest := fs.2 in
-      let rx := Re (rs !!! i) op' _ _ (x, σ) in
-      (rx.1, glob_St_recomp rest rx.2).
+      let rx := sReifier_re (rs !!! i) op' (x, σ) in
+      optionO_map (prodO_map idfun (gState_recomp rest)) rx.
+  Next Obligation. solve_proper_please. Qed.
 
-  Record in_hvec {n} (r : R) (rs : hvec n) : Type :=
-    { idx : fin n;
-      opF : Op r → Op (rs !!! idx);
-      inF {X} `{!Cofe X} (op : Op r) :
-        ofe_iso (In op ♯ X) (In (opF op) ♯ X);
-      outF {X} `{!Cofe X} (op : Op r) :
-        ofe_iso (Out op ♯ X) (Out (opF op) ♯ X);
-      stF  {X} `{!Cofe X} :
-        ofe_iso (St r ♯ X) (St (rs !!! idx) ♯ X);
-      reF {X} `{!Cofe X} (op : Op r) (x : In op ♯ X)
-          (y : Out op ♯ X) (s1 s2 : St r ♯ X) :
-        Re r op X _ (x, s1) ≡ (y, s2) →
-          Re (rs !!! idx) (opF op) X _ (ofe_iso_1 (inF op) x, ofe_iso_1 stF s1) ≡
-            (ofe_iso_1 (outF op) y, ofe_iso_1 stF s2)
-    }.
-  Arguments idx {_ _ _} _.
+  (** We can turn a collection of reifiers into a single reifier *)
+  Definition gReifiers_sReifier {n} (rs : gReifiers n) : sReifier :=
+    {| sReifier_ops := gReifiers_ops rs;
+       sReifier_state := gReifiers_state rs;
+       sReifier_re := @gReifiers_re n rs;
+    |}.
 
-  Definition in_hvec_op {n} {r : R} {rs : hvec n} (rin : in_hvec r rs)
-    (op : Op r) : glob_Op rs.
-  Proof.
-    refine (existT (idx rin) _).
-    apply (opF _ _ rin op).
-  Defined.
-  Definition in_hvec_in {n} {r : R} {rs : hvec n} (rin : in_hvec r rs)
-                        {X} `{Cofe X} (op : Op r)
-    (x : In op ♯ X) : glob_In (in_hvec_op rin op) ♯ X.
-  Proof.
-    unfold glob_In.
-    unfold in_hvec_op; simpl.
-    apply (ofe_iso_1 (inF _ _ _ _) x).
-  Defined.
-  Definition in_hvec_st {n} {r : R} {rs : hvec n} (rin : in_hvec r rs)
-                        {X} `{Cofe X} (op : Op r)
-    (x : St r ♯ X) : St (rs !!! idx rin) ♯ X.
-  Proof.
-    apply (ofe_iso_1 (stF _ _ _) x).
-  Defined.
-  Definition in_hvec_out {n} {r : R} {rs : hvec n} (rout : in_hvec r rs)
-                        {X} `{Cofe X} (op : Op r)
-    (x : Out op ♯ X) : glob_Out (in_hvec_op rout op) ♯ X.
-  Proof.
-    unfold glob_Out.
-    unfold in_hvec_op; simpl.
-    apply (ofe_iso_1 (outF _ _ _ _) x).
-  Defined.
+  (* XXX : move *)
+  Global Instance optionO_map_proper (A B : ofe) :
+    Proper ((≡) ==> (≡)) (@optionO_map A B).
+  Proof. solve_proper. Qed.
 
-  Lemma glob_Re_idx {n} (r : R) (rs : hvec n) (rin : in_hvec r rs)
-    {X} `{!Cofe X} (i : fin n) (op : Op (rs !!! i))
-    (x : In op ♯ X) (σ : St (rs !!! i) ♯ X) (rest : glob_St_rest i rs ♯ X) :
-    glob_Re (existT i op) (x,glob_St_recomp rest σ) ≡
-      prodO_map idfun (glob_St_recomp rest) $ Re (rs !!! i) op X _ (x,σ).
+  Lemma gReifiers_re_idx {n}  (i : fin n) (rs : gReifiers n)
+    {X} `{!Cofe X} (op : opid (sReifier_ops (rs !!! i)))
+    (x : Ins (sReifier_ops _ op) ♯ X)
+    (σ : sReifier_state (rs !!! i) ♯ X) (rest : gState_rest i rs ♯ X) :
+    gReifiers_re rs (existT i op) (x, gState_recomp rest σ) ≡
+      optionO_map (prodO_map idfun (gState_recomp rest))
+           (sReifier_re (rs !!! i) op (x,σ)).
   Proof.
-    Opaque glob_St_recomp.
-    unfold glob_Re. simpl.
-    trans (((Re (rs !!! i) op X _ (x, σ)).1, glob_St_recomp rest (Re (rs !!! i) op X _ (x, σ)).2)).
-    { repeat f_equiv; rewrite glob_St_decomp_recomp//. }
-    destruct (Re (rs !!! i) op X _ (x, σ)) as [y σ'].
-    simpl. reflexivity.
+    unfold gReifiers_re. cbn-[prodO_map optionO_map].
+    f_equiv; last repeat f_equiv.
+    - eapply optionO_map_proper.
+      intros [x1 x2]; simpl. f_equiv.
+      f_equiv. f_equiv.
+      rewrite gState_decomp_recomp//.
+    - rewrite gState_decomp_recomp//.
   Qed.
 
-  Lemma in_hvec_re {n} (r : R) (rs : hvec n) (rin : in_hvec r rs)
-                   {X} `{!Cofe X}
-                   (op : Op r) (x : In op ♯ X) (σ : St r ♯ X)
-                   (y : Out op ♯ X) (σ' : St r ♯ X)
-                   (rest : glob_St_rest (idx rin) rs ♯ X)
-    : Re r op X _ (x,σ) ≡ (y, σ') →
-      glob_Re (in_hvec_op rin op)
-        (in_hvec_in rin _ x,glob_St_recomp rest (in_hvec_st rin op σ))
-        ≡ (in_hvec_out rin _ y, glob_St_recomp rest (in_hvec_st rin op σ')).
+  Class subReifier {n} (r : sReifier) (rs : gReifiers n) :=
+    { sR_idx : fin n;
+      sR_ops :: subEff (sReifier_ops r) (sReifier_ops (rs !!! sR_idx));
+      sR_state  {X} `{!Cofe X} :
+        ofe_iso (sReifier_state r ♯ X) (sReifier_state (rs !!! sR_idx) ♯ X);
+      sR_re {X} `{!Cofe X} (op : opid (sReifier_ops r))
+        (x : Ins (sReifier_ops _ op) ♯ X)
+        (y : Outs (sReifier_ops _ op) ♯ X)
+        (s1 s2 : sReifier_state r ♯ X) :
+        sReifier_re r op (x, s1) ≡ Some (y, s2) →
+        sReifier_re (rs !!! sR_idx) (subEff_opid op)
+          (subEff_conv_ins x, ofe_iso_1 sR_state s1) ≡
+          Some (subEff_conv_outs y, ofe_iso_1 sR_state s2) }.
+
+  #[global] Instance subReifier_here {n} (r : sReifier) (rs : gReifiers n) :
+    subReifier r (gReifiers_cons r rs).
+  Proof.
+    simple refine ({| sR_idx := 0%fin |}).
+    - simpl. intros. apply iso_ofe_refl.
+    - intros X ? op x y s1 s2.
+      simpl. eauto.
+  Defined.
+  #[global] Instance subReifier_there {n} (r r' : sReifier) (rs : gReifiers n) :
+    subReifier r rs →
+    subReifier r (gReifiers_cons r' rs).
+  Proof.
+    intros SR.
+    simple refine ({| sR_idx := FS sR_idx |}).
+    - simpl. intros. apply sR_state.
+    - intros X ? op x y s1 s2.
+      simpl. apply sR_re.
+  Defined.
+
+  #[local] Definition subR_op {n} {r : sReifier} {rs : gReifiers n} `{!subReifier r rs} :
+    opid (sReifier_ops r) → opid (gReifiers_ops rs).
+  Proof.
+    intros op.
+    simpl.
+    refine (existT sR_idx (subEff_opid op)).
+  Defined.
+  Definition subR_conv_state {n} {r : sReifier} {rs : gReifiers n} `{!subReifier r rs}
+    {X} `{!Cofe X}:
+    (sReifier_state r ♯ X) -n> (sReifier_state (rs !!! sR_idx) ♯ X) :=
+    ofe_iso_1 sR_state.
+  Instance subReifier_subEff {n} {r : sReifier} {rs : gReifiers n} `{!subReifier r rs} :
+    subEff (sReifier_ops r) (gReifiers_ops rs).
+  Proof.
+    simple refine {| subEff_opid := subR_op |}.
+    - intros op X ?. simpl.
+      apply subEff_ins.
+    - intros op X ?. simpl.
+      apply subEff_outs.
+  Defined.
+
+  Lemma subReifier_reify {n} (r : sReifier)
+    (rs : gReifiers n) `{!subReifier r rs} {X} `{!Cofe X}
+    (op : opid (sReifier_ops r))
+    (x : Ins (sReifier_ops _ op) ♯ X) (y : Outs (sReifier_ops _ op) ♯ X)
+    (σ σ' : sReifier_state r ♯ X) (rest : gState_rest sR_idx rs ♯ X) :
+    sReifier_re r op (x,σ) ≡ Some (y, σ') →
+    gReifiers_re rs (subEff_opid op)
+      (subEff_conv_ins x, gState_recomp rest (subR_conv_state σ))
+      ≡ Some (subEff_conv_outs y, gState_recomp rest (subR_conv_state σ')).
   Proof.
     intros Hre.
-    apply (reF r rs rin) in Hre.
-    unfold in_hvec_op.
-    rewrite glob_Re_idx//.
+    apply sR_re in Hre.
+    rewrite gReifiers_re_idx//.
     rewrite Hre. simpl. reflexivity.
   Qed.
 
-End abstract_reseeee.
-
-
-Section reify.
-  Definition reify_eff (E : opsInterp) (stateF : oFunctor) :=
-    ∀ (op : opid E) (X : ofe) `{Cofe X},
-      ((Ins (E op) ♯ X) * (stateF ♯ X) -n> optionO ((Outs (E op) ♯ X) * (stateF ♯ X)))%type.
-
-  Record sReifier :=
-    { sReifier_ops : opsInterp;
-      sReifier_state : oFunctor;
-      sReifier_re : reify_eff sReifier_ops sReifier_state;
-      sReifier_inhab :: Inhabited (sReifier_state ♯ unitO);
-      sReifier_cofe X (HX : Cofe X) :: Cofe (sReifier_state ♯ X);
-    }.
-  Set Printing Universes.
-  About list. About Vector.t.
-  Coercion  sReifier_re : sReifier >-> Funclass.
-
-  Inductive gReifiers : nat → Type :=
-  | gReifiers_nil : gReifiers 0
-  | gReifiers_cons {n} : sReifier → gReifiers n → gReifiers (S n)
-  .
-
-  Fixpoint gReifiers_state {n} (rs : gReifiers n) : oFunctor :=
-    match rs with
-    | gReifiers_nil => unitO
-    | gReifiers_cons sR rs => sReifier_state sR * (gReifiers_state rs)
-    end.
-
-  Fixpoint gReifiers_ops {n} (rs : gReifiers n) : opsInterp :=
-    match rs with
-    | gReifiers_nil => opsInterp.nil
-    | gReifiers_cons sR rs => opsInterp.app (sReifier_ops sR) (gReifiers_ops rs)
-    end.
-
-  Definition grs_S_inv {n} (P : gReifiers (S n) → Type)
-    (Hcons : ∀ sR v, P (gReifiers_cons sR v)) v : P v.
-  Proof.
-    revert P Hcons.
-    refine match v with gReifiers_nil => tt
-                      | gReifiers_cons sR v => λ P Hcons, Hcons sR v end.
-  Defined.
-
-  Global Instance gReifiers_lookup_total : ∀ m, LookupTotal (fin m) sReifier (gReifiers m) :=
-  fix go m i {struct i} := let _ : ∀ m, LookupTotal _ _ _ := @go in
-  match i in fin m return gReifiers m → sReifier with
-  | 0%fin => grs_S_inv (λ _, sReifier) (λ x _, x)
-  | FS j => grs_S_inv (λ _, sReifier) (λ _ v, v !!! j)
-  end.
-
-  Fixpoint gReifiers_state_rest {m} (i : fin m) : gReifiers m → oFunctor :=
-    match i in fin m return gReifiers m → oFunctor with
-    | 0%fin => grs_S_inv (λ _, oFunctor)
-                 (λ sR rs, gReifiers_state rs)
-    | FS j => grs_S_inv (λ _, oFunctor)
-                 (λ sR rs, sReifier_state sR * gReifiers_state_rest j rs)%OF
-    end.
-
-  Lemma rs_state_decomp {m} (i : fin m) (rs : gReifiers m) {X} `{!Cofe X} :
-    ofe_iso ((sReifier_state (rs !!! i) ♯ X) * (gReifiers_state_rest i rs ♯ X))%type
-            (gReifiers_state rs ♯ X).
-  Proof.
-    revert i. induction rs as [|? [F stateF re ? ?] rs]=>i.
-    { inversion i. }
-    inv_fin i; simpl.
-    { apply iso_ofe_refl. }
-    intros i.
-    specialize (IHrs i).
-    unshelve esplit.
-    - simple refine (λne sxr, let r' := ofe_iso_1 IHrs (sxr.1,sxr.2.2) in
-                              (sxr.2.1, r')).
-      solve_proper.
-    - simple refine (λne xr, let sr := ofe_iso_2 IHrs (xr.2) in
-                             (sr.1,(xr.1,sr.2))).
-      solve_proper.
-    - intros (x & r). simpl. f_equiv.
-      rewrite -surjective_pairing. apply ofe_iso_12.
-    - intros (s & x & r). simpl. repeat f_equiv; rewrite ofe_iso_21//.
-  Qed.
-
-  #[export] Instance reifiers_state_cofe {n} (rs : gReifiers n) X `{!Cofe X} :
-    Cofe (gReifiers_state rs ♯ X).
-  Proof.
-    induction rs; simpl; first apply _.    destruct s. apply _.
-  Qed.
-  #[export] Instance reifiers_state_inhab {n} (rs : gReifiers n) :
-    Inhabited (gReifiers_state rs ♯ unitO).
-  Proof.
-    induction rs; simpl; first apply _.
-    destruct s. apply _.
-  Qed.
-
-  Definition reifiers_op_idx' {n} (rs : gReifiers n)
-    (op : opid (gReifiers_ops rs)) :
-    { i : fin n & opid (sReifier_ops (rs !!! i)) }.
-  Proof.
-    induction rs as [|? sR rs].
-    { apply Empty_set_rect. exact op. }
-    simpl in op.
-    destruct op as [op|op]; simpl.
-    - refine (existT 0%fin op).
-    - pose (i := projT1 (IHrs op)).
-      exact (existT (FS i) (projT2 (IHrs op))).
-  Defined.
-  Definition reifiers_op_idx {n} (rs : gReifiers n)
-    (op : opid (gReifiers_ops rs)) : fin n
-    := projT1 $ reifiers_op_idx' rs op.
-  Definition reifiers_op_conv {n} (rs : gReifiers n)
-    (op : opid (gReifiers_ops rs)) : opid (sReifier_ops (rs !!! reifiers_op_idx rs op))
-    := projT2 $ reifiers_op_idx' rs op.
-  Lemma reifiers_op_idx_0 {n} (sR : sReifier) (rs : gReifiers n)
-    (op : opid (sReifier_ops sR)) :
-    reifiers_op_idx (gReifiers_cons sR rs) (inl op) = 0%fin.
-  Proof. reflexivity. Qed.
-  Lemma reifiers_op_idx_S {n} (sR : sReifier) (rs : gReifiers n)
-    (op : opid (gReifiers_ops rs)) :
-    reifiers_op_idx (gReifiers_cons sR rs) (inr op) = FS $ reifiers_op_idx rs op.
-  Proof. reflexivity. Qed.
-
-  (* those are just identities? *)
-  Definition reifiers_op_conv_ins {n} (rs : gReifiers n)
-    (op : opid (gReifiers_ops rs)) {X} `{!Cofe X}:
-    ofe_iso (Ins (gReifiers_ops rs op) ♯ X)
-      (Ins (sReifier_ops (rs !!! (reifiers_op_idx rs op)) (reifiers_op_conv rs op)) ♯ X).
-  Proof.
-    induction rs as [|? [F stateF re ? ?] rs].
-    { apply Empty_set_rect. exact op. }
-    simpl in op.
-    destruct op as [op|op].
-    - unfold reifiers_op_conv. simpl.
-      apply iso_ofe_refl.
-    - simpl. unfold reifiers_op_conv.
-      apply IHrs.
-  Defined.
-  Definition reifiers_op_conv_outs {n} (rs : gReifiers n)
-    (op : opid (gReifiers_ops rs)) {X} `{!Cofe X}:
-    ofe_iso (Outs (gReifiers_ops rs op) ♯ X)
-      (Outs (sReifier_ops (rs !!! (reifiers_op_idx rs op)) (reifiers_op_conv rs op)) ♯ X).
-  Proof.
-    induction rs as [|? [F stateF re ? ?] rs].
-    { apply Empty_set_rect. exact op. }
-    simpl in op.
-    destruct op as [op|op].
-    - unfold reifiers_op_conv. simpl.
-      apply iso_ofe_refl.
-    - simpl. unfold reifiers_op_conv.
-      apply IHrs.
-  Defined.
-
-  Program Definition reifiers_op_conv_state {n} {i : fin n} {rs : gReifiers n}
-   {X} `{!Cofe X} :
-    (rs_state_rest i rs ♯ X) -n>
-    (sReifier_state (rs !!! i) ♯ X) -n>
-      gReifiers_state rs ♯ X :=
-    λne rest σ1,  ofe_iso_1 (rs_state_decomp i rs) (σ1,rest).
-  Solve All Obligations with solve_proper_please.
-
-  Program Definition reifiers_op_conv_state' {n} (i : fin n) {rs : gReifiers n}
-    {X} `{!Cofe X} :
-    gReifiers_state rs ♯ X -n>
-      (prodO (sReifier_state (rs !!! i) ♯ X) (rs_state_rest i rs ♯ X))
-    := ofe_iso_2 (rs_state_decomp i rs).
-
-  Definition reifiers_re_idx {n} (i : fin n) (rs : gReifiers n)
-    (op : opid (sReifier_ops (rs !!! i))) (X : ofe) `{Cofe X} :
-    ((Ins (sReifier_ops (rs !!! i) op) ♯ X) * (gReifiers_state rs ♯ X)
-     → optionO ((Outs (sReifier_ops (rs !!! i) op) ♯ X) * (gReifiers_state rs ♯ X)))%type.
-  Proof.
-    intros [inp s].
-    set (σ := fst (reifiers_op_conv_state' i s)).
-    set (rest := snd (reifiers_op_conv_state' i s)).
-    simple refine (optionO_map (prodO_map idfun (reifiers_op_conv_state rest)) (sReifier_re (rs !!! i) op X _ (inp, σ))).
-  Defined.
-
-  #[global] Instance reifiers_re_idx_ne  {n} (i : fin n) (rs : gReifiers n)
-    (op : opid (sReifier_ops (rs !!! i))) (X : ofe) `{Cofe X} :
-    NonExpansive (reifiers_re_idx i rs op X).
-  Proof.
-    intros m [i1 s1] [i2 s2] [Hi Hs].
-    unfold reifiers_re_idx. repeat f_equiv; eauto.
-  Qed.
-
-  (* Definition reifiers_re {n} (rs : gReifiers n) *)
-  (*   (op : opid (gReifiers_ops rs)) (X : ofe) `{Cofe X} : *)
-  (*   ((Ins (gReifiers_ops rs op) ♯ X) * (gReifiers_state rs ♯ X) *)
-  (*    → optionO ((Outs (gReifiers_ops rs op) ♯ X) * (gReifiers_state rs ♯ X)))%type. *)
-  (* Proof. *)
-  (*   intros xs. *)
-  (*   refine *)
-  (*     (optionO_map (prodO_map (ofe_iso_2 (reifiers_op_conv_outs rs op)) idfun) $ reifiers_re_idx (reifiers_op_idx rs op) rs (reifiers_op_conv rs op) X *)
-  (*        (ofe_iso_1 (reifiers_op_conv_ins rs op) xs.1, xs.2)). *)
-  (* Defined. *)
-  Definition reifiers_re {n} (rs : gReifiers n)
-    (op : opid (gReifiers_ops rs)) (X : ofe) `{Cofe X} :
-    ((Ins (gReifiers_ops rs op) ♯ X) * (gReifiers_state rs ♯ X)
-     → optionO ((Outs (gReifiers_ops rs op) ♯ X) * (gReifiers_state rs ♯ X)))%type.
-  Proof.
-    induction rs as [|? sR rs].
-    { inversion op. }
-    simpl in op.
-    destruct op as [op|op]; cbn-[oFunctor_apply].
-    - intros [x [s1 s2]].
-      apply (option_map (prod_map idfun (λ s1', (s1',s2))) (sReifier_re sR op X _ (x,s1))).
-    - intros [x [s1 s2]].
-      apply
-        (option_map (prod_map idfun (λ s2', (s1,s2'))) (IHrs _ (x,s2))).
-  Defined.
-
-
-  #[global] Instance reifiers_re_ne {n} (rs : gReifiers n)
-       (op : opid (gReifiers_ops rs)) (X : ofe) `{Cofe X} :
-    NonExpansive (reifiers_re rs op X).
-  Proof.
-    (* unfold reifiers_re. solve_proper_please. *)
-  Admitted.
-  #[global] Instance reifiers_re_proper  {n} (rs : gReifiers n)
-       (op : opid (gReifiers_ops rs)) (X : ofe) `{Cofe X} :
-    Proper ((≡) ==> (≡)) (reifiers_re rs op X).
-  Proof. apply ne_proper. apply _. Qed.
-
-  (* Class inReifier {n} (sR : sReifier) (rs : gReifiers n) := *)
-  (*   { inR_idx : fin n; *)
-  (*     inR_lookup : rs !!! inR_idx = sR *)
-  (*   }. *)
-  Class inReifier {n} (sR : sReifier) (rs : gReifiers n) :=
-    { inR_idx : fin n;
-      inR_sub :: subEff (sReifier_ops sR) (sReifier_ops (rs !!! inR_idx));
-      inR_state X `{!Cofe X} :
-         ofe_iso (sReifier_state sR ♯ X)
-                 (sReifier_state (rs !!! inR_idx) ♯ X);
-      inR_reify X `{!Cofe X} (op : opid (sReifier_ops sR))
-          (x : Ins (sReifier_ops sR op) ♯ X)
-          (s : sReifier_state sR ♯ X) :
-      let x' : Ins (sReifier_ops (rs !!! inR_idx) (subEff_opid op)) ♯ X
-        := subEff_conv_ins x in
-      let s' : sReifier_state (rs !!! inR_idx) ♯ X
-        := ofe_iso_1 (inR_state X) s in
-         sReifier_re sR op X _ (x , s) ≡
-         optionO_map (prodO_map subEff_conv_outs2 (ofe_iso_2 (inR_state X))) $
-           sReifier_re (rs !!! inR_idx) (subEff_opid op) X _ (x', s')
-    }.
-  Definition inReifier_st_conv {n} {sR} {rs : gReifiers n} `{!inReifier sR rs}
-    {X} `{!Cofe X}:
-    sReifier_state sR ♯ X -n> sReifier_state (rs !!! inR_idx) ♯ X
-    := ofe_iso_1 (inR_state X).
-  Definition inReifier_st_conv2 {n} {sR} {rs : gReifiers n} `{!inReifier sR rs}
-    {X} `{!Cofe X}:
-    sReifier_state (rs !!! inR_idx) ♯ X -n> sReifier_state sR ♯ X
-    := ofe_iso_2 (inR_state X).
-
-  (* Program Definition sRs_transport {A B : sReifier} (H : A = B) *)
-  (*   {X} `{!Cofe X} : *)
-  (*   ofe_iso (sReifier_state A ♯ X) (sReifier_state B ♯ X) *)
-  (*   := eq_rect A (λ B, ofe_iso (sReifier_state B ♯ X) (sReifier_state B ♯ X)) *)
-  (*        iso_ofe_refl B H. *)
-  (* Next Obligation. solve_proper. Qed. *)
-
-  (* Definition sReq_opid {A B : sReifier} (H : A = B) : *)
-  (*   opid (sReifier_ops A) = opid (sReifier_ops B). *)
-  (* Proof. *)
-  (*   induction H. reflexivity. *)
-  (* Defined. *)
-  (* Definition sRop_transport {A B : sReifier} (H : A = B) : *)
-  (*   opid (sReifier_ops A) → opid (sReifier_ops B). *)
-  (* Proof. *)
-  (*   induction H. exact id. *)
-  (* Defined. *)
-
-  (* Definition inR_opid {n} {sR} (rs : gReifiers n) {i : fin n} *)
-  (*   (Hi : rs !!! i = sR): *)
-  (*   opid (sReifier_ops sR) → opid (gReifiers_ops rs). *)
-  (* Proof. *)
-  (*   induction rs as [|? sR' rs]. *)
-  (*   { inversion i. } *)
-  (*   inv_fin i. *)
-  (*   { simpl. intros Hsr. *)
-  (*     refine (inl ∘ sRop_transport (eq_sym Hsr)). } *)
-  (*   intros i. simpl. intros Hi. *)
-  (*   refine (inr ∘ IHrs i Hi). *)
-  (* Defined. *)
-
-  (* Definition subEff_transp {sR sR'} (H : sR = sR') : *)
-  (*   subEff (sReifier_ops sR) (sReifier_ops sR'). *)
-  (* Proof. *)
-  (*   refine {| subEff_opid := sRop_transport H |}. *)
-  (*   - intros. *)
-  (*     assert ((sReifier_ops sR op) = (sReifier_ops sR' (sRop_transport H op))). *)
-  (*     { *)
-  (*       rewrite sReq_opid. *)
-  (*     intros op X HX. *)
-  #[global] Instance inR_subEff' {n} (i : fin n) (rs : gReifiers n) :
-    subEff (sReifier_ops (rs !!! i)) (gReifiers_ops rs).
-  Proof.
-    induction rs as [|? sR' rs].
-    { inversion i. }
-    inv_fin i.
-    { simpl. apply _. }
-    intros i. simpl.
-    apply subEff_app_r.
-    apply IHrs.
-  Defined.
-
-  Definition subEff_comp E1 E2 E3 :
-    subEff E1 E2 → subEff E2 E3 → subEff E1 E3.
-  Proof.
-    intros H1 H2.
-    simple refine
-             {| subEff_opid (op : opid E1) := subEff_opid (subEff_opid op) |}.
-    - intros.
-      eapply iso_ofe_trans.
-      + apply subEff_ins.
-      + apply subEff_ins.
-    - intros.
-      eapply iso_ofe_trans.
-      + apply subEff_outs.
-      + apply subEff_outs.
-  Defined.
-
-  #[global] Instance inR_subEff {n} sR (rs : gReifiers n) :
-    inReifier sR rs → subEff (sReifier_ops sR) (gReifiers_ops rs).
-  Proof.
-    intros HR.
-    eapply subEff_comp.
-    - apply HR.
-    - apply inR_subEff'.
-  Defined.
-
-  Global Instance optionO_map_proper A B f :
-    Proper ((≡) ==> (≡)) (@optionO_map A B f).
-  Proof. apply ne_proper. apply _. Qed.
-
-
-  (* XXX: see why sReifier_re does not work as a good coercion here *)
-  Lemma inR_subreify {n} sR (rs : gReifiers n)
-   {inR0 : inReifier sR rs}
-    {X} `{!Cofe X}
-    (σ : sReifier_state sR ♯ X)
-    (rest : rs_state_rest inR_idx rs ♯ X)
-    (op : opid (sReifier_ops sR))
-    (i : Ins (sReifier_ops sR op) ♯ X)
-    :
-    let σ1 := inReifier_st_conv σ in
-    let fs1 := reifiers_op_conv_state rest σ1 in
-    reifiers_re rs (subEff_opid op) X (ofe_iso_1 (subEff_ins op) i, fs1) ≡
-     optionO_map (prodO_map subEff_conv_outs (reifiers_op_conv_state rest ◎ inReifier_st_conv))
-      (sReifier_re sR op X _ (i, σ)).
-  Proof.
-    intros σ1.
-    set (i' := subEff_conv_ins i).
-    intros fs1.
-    assert (sReifier_re sR op X _ (i,σ) ≡
-       optionO_map (prodO_map subEff_conv_outs2 inReifier_st_conv2)
-       (sReifier_re (rs !!! inR_idx) (subEff_opid op) X _ (i', σ1))) as Heq.
-    { apply inR_reify. }
-    pose (op1 :=  (@subEff_opid (sReifier_ops sR) (sReifier_ops (rs !!! @inR_idx n sR rs inR0))) inR_sub op).
-    fold op1 in Heq.
-    pose  (op' := @subEff_opid _ (@gReifiers_ops n rs)
-                    (@inR_subEff' n _ rs) op1).
-    change (@subEff_opid (sReifier_ops sR) (@gReifiers_ops n rs) (@inR_subEff n sR rs inR0) op) with op'.
-    induction rs as [|? sR' rs].
-    { pose (j:= inR_idx). inversion j. }
-    simpl in op'. 
-    remember op' as op2.
-    Set Printing All.
-    Etrans. 2:{
-            apply optionO_map_proper.
-            symmetry. apply Heq. }
-          unfold reifiers_re. simpl fst. simpl snd.
-    pose (op1 :=  (@subEff_opid (sReifier_ops sR) (sReifier_ops (rs !!! @inR_idx n sR rs inR0))) inR_sub op).
-    fold op1.
-    pose  (op' := @subEff_opid _ (@gReifiers_ops n rs)
-                    (@inR_subEff' n _ rs) op1).
-Set Printing Implicit.
-    fold op'.
-    induction rs as [|? sR' rs].
-    { pose (j:= inR_idx). inversion j. }
-    simpl in op'.
-    destruct op' as [op'|op'].
-    simpl reifiers_op_idx.
-    simpl.
-    unfold reifiers_re. simpl.
-    
-    set ().
-    set (| 
-    Check .
-    
-    : let σ1 := ofe_iso_2 (sRs_transport inR_lookup) σ in
-      let fs1 := reifiers_op_conv_state rest σ1 in
-   reifiers_re rs (subEff_opid op) X (ofe_iso_1 (subEff_ins op) i, fs1) ≡
-   optionO_map (prodO_map (ofe_iso_1 (subEff_outs op)) (reifiers_op_conv_state rest ◎ ofe_iso_2 (sRs_transport inR_lookup)))
-     (sReifier_re sR op X _ (i, σ)).
-  Proof.
-    revert op i σ rest.
-    induction rs as [|? sR' rs]=>op i σ rest.
-    { destruct inR0.
-      inversion inR_idx0. }
-    pose (HH := inR_subEff _ _ inR0).
-    destruct inR0.
-    inv_fin inR_idx0.
-    { intros Heq rest HH.
-      simpl in Heq.
-      unfold reifiers_re.
-      Set Printing Implicit.
-      simpl subEff_opid.
-      assert (reifiers_op_idx rs op)
-      simpl.
-      generalize (@subEff_opid (sReifier_ops sR) (@gReifiers_ops (S n) (@gReifiers_cons n sR1 rs))
-       (@inR_subEff (S n) sR (@gReifiers_cons n sR1 rs)
-          {| inR_idx := 0%fin; inR_lookup := Heq |}) op).
-      generalize (subEff_opid op : opid (gReifiers_ops (gReifiers_cons sR1 rs))).
-      simpl reifiers_re.
-      destruct  as [op1|op1].
-    Set Printing All.
-
-      simpl.
-Eval simpl in . 
-      simpl reifiers_re.
-      unfold inR_conv_state.
-      simpl inR_conv_state.
-      simpl.
-
-      
-[F stateF re ? ?]
-    s
-    set fs1 := inR_conv_state rest σ.
-    refine (reifiers_re rs (subEff_opid op) X (ofe_iso_1 (subEff_ins op) i,fs1) = _).
-    refine (optionO_map _ (sReifier_re sR op X _ (i,σ))).
-    refine (prodO_map (ofe_iso_1 (subEff_outs op)) _).
-    apply (inR_conv_state rest).
-    Show Proof.
-    refine (_ ◎ _); last first.
-    + apply (sRs_transport (eq_sym inR_lookup)).
-    + refine (λne σ2, ofe_iso_1 (rs_state_decomp inR_idx rs) (σ2, rest)).
-      solve_proper.
-        Show Proof.
-      subR_reify (op : opid F) X `{Cofe X}
-        (i : Ins (F op) ♯ X) (s : stateF ♯ X) (s_rest : rest ♯ X) :
-        let i' := subEff_conv_ins i in
-        let s' := subState_conv_state s_rest s in
-        reifiers_re rs (subEff_opid op) X (i',s') ≡
-          optionO_map (prodO_map subEff_conv_outs (subState_conv_state s_rest))
-                      (re op X _ (i,s))
-
-               
+  (************************************************************************)
 
   Context {n : nat} (rs : gReifiers n).
   Notation F := (gReifiers_ops rs).
   Notation stateF := (gReifiers_state rs).
   Notation IT := (IT F).
   Notation ITV := (ITV F).
+  Implicit Type op : opid F.
+  Implicit Type α β : IT.
 
-  Notation stateM := ((stateF ♯ IT -n> (stateF ♯ IT) * IT))%type.
+  Notation stateM := ((stateF ♯ IT -n> (stateF ♯ IT) * IT)).
   #[local] Instance stateT_inhab : Inhabited stateM.
   Proof.
     simple refine (populate (λne s, (s, inhabitant))).
@@ -657,7 +265,7 @@ Eval simpl in .
   Proof.
     simpl.
     simple refine (λne i (k : _ -n> _) (s : stateF ♯ IT), _).
-    - simple refine (let ns := reifiers_re rs op _ (oFunctor_map _ (inlO,fstO) i, s) in _).
+    - simple refine (let ns := gReifiers_re rs op (oFunctor_map _ (inlO,fstO) i, s) in _).
       simple refine (from_option (λ ns,
                          let out2' := k $ oFunctor_map (Outs (F op)) (fstO,inlO) ns.1 in
                          (ns.2, Tau $ laterO_map fstO out2'))
@@ -712,7 +320,7 @@ Eval simpl in .
   Qed.
 
   Lemma reify_vis_eq op i o k σ σ' :
-    reifiers_re rs op _ (i,σ) ≡ Some (o,σ') →
+    gReifiers_re rs op (i,σ) ≡ Some (o,σ') →
     reify (Vis op i k) σ ≡ (σ', Tau $ k o).
   Proof.
     intros Hst.
@@ -723,11 +331,11 @@ Eval simpl in .
     { f_equiv.
       apply IT_rec1_vis. }
     Opaque prod_in. simpl.
-    pose (r := (reifiers_re rs op _
+    pose (r := (gReifiers_re rs op
       (oFunctor_map (Ins (F op)) (inlO, fstO)
                     (oFunctor_map (Ins (F op)) (sumO_rec idfun unreify, prod_in idfun reify) i), σ))).
     fold r.
-    assert (r ≡ reifiers_re rs op _ (i,σ)) as Hr'.
+    assert (r ≡ gReifiers_re rs op (i,σ)) as Hr'.
     { unfold r. f_equiv. f_equiv.
       rewrite -oFunctor_map_compose.
       etrans; last by apply oFunctor_map_id.
@@ -751,11 +359,12 @@ Eval simpl in .
     repeat f_equiv.
     { intro; done. }
     etrans; last by apply oFunctor_map_id.
+    simpl.
     repeat f_equiv; intro; done.
   Qed.
 
   Lemma reify_vis_None op i k σ :
-    reifiers_re rs op _ (i,σ) ≡ None →
+    gReifiers_re rs op (i,σ) ≡ None →
     reify (Vis op i k) σ ≡ (σ, Err RuntimeErr).
   Proof.
     intros Hs.
@@ -766,11 +375,11 @@ Eval simpl in .
     { f_equiv.
       apply IT_rec1_vis. }
     simpl.
-    pose (r := (reifiers_re rs op _
+    pose (r := (gReifiers_re rs op
       (oFunctor_map (Ins (F op)) (inlO, fstO)
                     (oFunctor_map (Ins (F op)) (sumO_rec idfun unreify, prod_in idfun reify) i), σ))).
     fold r.
-    assert (r ≡ reifiers_re rs op _ (i,σ)) as Hr'.
+    assert (r ≡ gReifiers_re rs op (i,σ)) as Hr'.
     { unfold r. f_equiv. f_equiv.
       rewrite -oFunctor_map_compose.
       etrans; last by apply oFunctor_map_id.
@@ -795,7 +404,7 @@ Eval simpl in .
     (reify (Vis op i k1) σ1 ≡ (σ2, Tick β) ⊢
      reify (Vis op i (laterO_map k2 ◎ k1)) σ1 ≡ (σ2, Tick (k2 β)) : PROP)%I.
   Proof.
-    destruct (reifiers_re rs op _ (i,σ1)) as [[o σ2']|] eqn:Hre; last first.
+    destruct (gReifiers_re rs op (i,σ1)) as [[o σ2']|] eqn:Hre; last first.
     - rewrite reify_vis_None; last by rewrite Hre//.
       iIntros "Hr". iExFalso.
       iPoseProof (prod_equivI with "Hr") as "[_ Hk]".
@@ -818,7 +427,7 @@ Eval simpl in .
      ⊢ ∃ α, reify (Vis op i k1) σ1 ≡ (σ2, Tick α) ∧ ▷ (β ≡ k2 α)
       : PROP)%I.
   Proof.
-    destruct (reifiers_re rs op _ (i,σ1)) as [[o σ2']|] eqn:Hre; last first.
+    destruct (gReifiers_re rs op (i,σ1)) as [[o σ2']|] eqn:Hre; last first.
     - rewrite reify_vis_None; last by rewrite Hre//.
       iIntros "Hr". iExFalso.
       iPoseProof (prod_equivI with "Hr") as "[_ Hk]".
@@ -845,10 +454,10 @@ Eval simpl in .
         iNext. by iApply internal_eq_sym.
   Qed.
 
-  Lemma reify_is_always_a_tick i op k σ β σ' :
-    reify (Vis i op k) σ ≡ (σ', β) → (∃ β', β ≡ Tick β') ∨ (β ≡ Err RuntimeErr).
+  Lemma reify_is_always_a_tick op x k σ β σ' :
+    reify (Vis op x k) σ ≡ (σ', β) → (∃ β', β ≡ Tick β') ∨ (β ≡ Err RuntimeErr).
   Proof.
-    destruct (reifiers_re rs i _ (op, σ)) as [[o σ'']|] eqn:Hre; last first.
+    destruct (gReifiers_re rs op (x, σ)) as [[o σ'']|] eqn:Hre; last first.
     - rewrite reify_vis_None; last by rewrite Hre//.
       intros [_ ?]. by right.
     - rewrite reify_vis_eq;last by rewrite Hre.
@@ -859,111 +468,5 @@ Eval simpl in .
       rewrite -Hlb. symmetry. apply Ho.
   Qed.
 
-End reify.
+End reifiers.
 Arguments reify {n} rs.
-
-
-
-Class subState {E : opsInterp}
-  (stateF : oFunctor) (rs : reifiers E) (rest : oFunctor) :=
-  SubState
-    { subS_decomp X `{Cofe X} :
-         ofe_iso (reifiers_state rs ♯ X) ((stateF * rest) ♯ X);
-    }.
-Program Definition subState_conv_state {E} {stateF : oFunctor} {rs : reifiers E} `{!subState stateF rs rest} {X} `{!Cofe X} :
-  (rest ♯ X) -n> (stateF ♯ X) -n> reifiers_state rs ♯ X :=
-  λne rst s, ofe_iso_2 (subS_decomp _) (s,rst).
-Solve Obligations with solve_proper.
-
-#[export] Instance subState_here {F E} (stateF : oFunctor) (re : reify_eff F stateF)
-  `{!Inhabited (stateF ♯ unitO)} `{forall X (HX : Cofe X), Cofe (stateF ♯ X)}
-  (rs : reifiers E) : subState stateF (reifiers_cons F stateF re rs) (reifiers_state rs).
-Proof.
-  split. simpl. intros X HX. apply iso_ofe_refl.
-Defined.
-
-#[export] Instance subState_there {F E E'} {stateF stateE} (reE : reify_eff E stateE)
-  (reF : reify_eff F stateF)
-  `{!Inhabited (stateF ♯ unitO)} `{forall X (HX : Cofe X), Cofe (stateF ♯ X)}
-  `{!Inhabited (stateE ♯ unitO)} `{forall X (HX : Cofe X), Cofe (stateE ♯ X)}
-  (rs : reifiers E')
-  `{!subState stateF rs rest}
-  : subState stateF (reifiers_cons E stateE reE rs) (stateE * rest).
-Proof.
-  split. cbn-[oFunctor_apply].
-  intros X HX.
-  unshelve esplit.
-  - simple refine (λne sx, let y := ofe_iso_1 (subS_decomp _) sx.2 in
-                           (y.1, (sx.1,y.2))).
-    + apply _.
-    + solve_proper.
-  - simple refine (λne fer, let y := ofe_iso_2 (subS_decomp _) (fer.1,fer.2.2) in
-                            (fer.2.1,y)).
-    + apply _.
-    + solve_proper.
-  - intros (f & e & r). simpl. rewrite ofe_iso_12. done.
-  - intros (e & r). simpl. f_equiv.
-    rewrite -surjective_pairing.
-    rewrite ofe_iso_21. done.
-Defined.
-
-Class subReifier {F E : opsInterp} {stateF}
-  (re : reify_eff F stateF) (rs : reifiers E) (rest : oFunctor) :=
-  SubReifier
-    { subR_subEff :: subEff F E;
-      subR_subS   :: subState stateF rs rest;
-      subR_reify (op : opid F) X `{Cofe X}
-        (i : Ins (F op) ♯ X) (s : stateF ♯ X) (s_rest : rest ♯ X) :
-        let i' := subEff_conv_ins i in
-        let s' := subState_conv_state s_rest s in
-        reifiers_re rs (subEff_opid op) X (i',s') ≡
-          optionO_map (prodO_map subEff_conv_outs (subState_conv_state s_rest))
-                      (re op X _ (i,s))
-    }.
-
-#[export] Instance subReifier_here {F E} {stateF} (re : reify_eff F stateF)
-  `{!Inhabited (stateF ♯ unitO)} `{forall X (HX : Cofe X), Cofe (stateF ♯ X)}
-  (rs : reifiers E) : subReifier re (reifiers_cons F stateF re rs) (reifiers_state rs).
-Proof.
-  esplit; try apply _.
-  intros op X HX i s rest. simpl.
-  destruct (re op X HX (i, s)) as [[o s']|] eqn:Hre;
-    rewrite Hre; reflexivity.
-Defined. (* we need it to be able to simplify .. *)
-
-#[export] Instance subReifier_there {F E E'} {stateF stateE}
-  (reE : reify_eff E stateE)
-  (reF : reify_eff F stateF)
-  `{!Inhabited (stateF ♯ unitO)} `{forall X (HX : Cofe X), Cofe (stateF ♯ X)}
-  `{!Inhabited (stateE ♯ unitO)} `{forall X (HX : Cofe X), Cofe (stateE ♯ X)}
-  (rs : reifiers E')
-  `{!subReifier reF rs rest}
-  : subReifier reF (reifiers_cons E stateE reE rs) (stateE * rest).
-Proof.
-  unshelve esplit.
-  { eapply subState_there; eauto. apply _. } (** XXX: why does typeclass search fail? *)
-  intros op X HX i s s_rest.
-  destruct (subState_conv_state s_rest s) as [sE' sR] eqn:Hdecomp.
-  destruct s_rest as [sE s_rest].
-  simpl in Hdecomp.
-  simplify_eq/=.
-  change (ofe_iso_2 (subS_decomp X) (s, s_rest)) with (subState_conv_state s_rest s).
-  assert
-    (reifiers_re rs (subEff_opid op) X (subEff_conv_ins i, subState_conv_state s_rest s) ≡ optionO_map (prodO_map subEff_conv_outs (subState_conv_state s_rest))
-       (reF op X HX (i, s))) as HH.
-  { apply subR_reify. }
-  revert HH.
-  destruct (reF op X HX (i, s)) as [[o s']|] eqn:HreF; simpl.
-  - destruct (reifiers_re rs (subEff_opid op) X
-                (subEff_conv_ins i, subState_conv_state s_rest s))
-      as [[o' s'_rest]|] eqn:Hre.
-    + rewrite Hre. simpl. intros [Ho Hs]%Some_equiv_inj%pair_equiv_inj.
-      solve_proper.
-    + rewrite Hre. simpl. inversion 1.
-  - destruct (reifiers_re rs (subEff_opid op) X
-                (subEff_conv_ins i, subState_conv_state s_rest s))
-      as [[o' s'_rest]|] eqn:Hre.
-    + rewrite Hre. simpl. inversion 1.
-    + rewrite Hre. simpl. done.
-Defined. (* ditto *)
-
